updates for documentation

Proofs/Refine_AC_A.thy
@@ -14,22 +14,46 @@ definition trusted_boot :: "nat \<Rightarrow> unit E_monad"
        
 context sable_m
 begin
+
+section {* Correspondence Example *}
+  
+text {* In this lemma, we establish that our lifted C implementation of
+\texttt{read\_passphrase()} corresponds to the same definition in our abstract
+specification. The \texttt{read\_passphrase()} reads the configuration pass
+phrase from the TPM chip's NVRAM, and returns it as an unpacked structured of
+type \texttt{TPM\_STORED\_DATA12}, according to the TCG standard. The abstract
+function is very simple. It simply calls the abstract TPM driver function
+\textsf{TPM\_NV\_ReadValue} and returns. The C implementation is more complex. It also
+calls the C implementation \texttt{TPM\_NV\_ReadValue()}, but it then must verify
+that the call to the driver succeeded and, if so, unpack the retrieved data
+structure containing the passphrase. *}
   
 lemma read_passphrase_corres:
-  "corres (R_STORED_DATA_rel string_rel) \<top> \<top> (read_passphrase i) (read_passphrase' (of_nat i))"
+  "corres (R_STORED_DATA_rel string_rel) \<top> \<top> (read_passphrase i)
+                                              (read_passphrase' (of_nat i))"
   (is "corres ?r _ _ _ _")
 unfolding read_passphrase_def read_passphrase'_def
 proof simp
   let ?r' = "R_HEAP_DATA_rel (E_STORED_DATA_rel string_rel)"
-  show "corres ?r \<top> \<top> (TPM_NV_ReadValue i 0 None)
-       (do ret' \<leftarrow> TPM_NV_ReadValue' (of_nat i) 0 0x190 (TPM_AUTHDATA_option_C (tdTPM_AUTHDATA_C (ARRAY _. 0)) 0) NULL;
-         condition (\<lambda>s. error_C (HEAP_DATA_exception_C.exception_C ret') \<noteq> 0)
-           (return (TPM_STORED_DATA12_exception_C (HEAP_DATA_exception_C.exception_C ret')
+  show "corres ?r \<top> \<top> 
+       (* Abstract read_passphrase *)
+       (TPM_NV_ReadValue i 0 None)
+       (* AutoCorres lifted read_passphrase() *)
+       (do ret' \<leftarrow> TPM_NV_ReadValue' (of_nat i) 0 0x190
+               (TPM_AUTHDATA_option_C
+                  (tdTPM_AUTHDATA_C (ARRAY _. 0)) 0) NULL;
+         condition
+           (\<lambda>s. error_C (HEAP_DATA_exception_C.exception_C ret') \<noteq> 0)
+           (return (TPM_STORED_DATA12_exception_C
+                (HEAP_DATA_exception_C.exception_C ret')
               (tdTPM_STORED_DATA12_C 0 0 0 NULL 0 NULL)))
            (do ret' \<leftarrow>
-               unpack_TPM_STORED_DATA12' (tdHEAP_DATA_C.data_C (HEAP_DATA_exception_C.value_C ret'))
-                (tdHEAP_DATA_C.dataSize_C (HEAP_DATA_exception_C.value_C ret'));
-               return (TPM_STORED_DATA12_exception_C (tdEXCEPTION_C NONE) ret')
+               unpack_TPM_STORED_DATA12' (tdHEAP_DATA_C.data_C 
+                      (HEAP_DATA_exception_C.value_C ret'))
+                (tdHEAP_DATA_C.dataSize_C
+                   (HEAP_DATA_exception_C.value_C ret'));
+               return (TPM_STORED_DATA12_exception_C
+                         (tdEXCEPTION_C NONE) ret')
             od)
       od)" (is "corres ?r _ _ ?read (?read' >>= ?d)")
   apply (rule corres_bind_return)
@@ -44,44 +68,56 @@ proof simp
       case (Inl e)
       fix s'
       assume "?r' rv (rv', s')"
-      with Inl have rv': "error_C (HEAP_DATA_exception_C.exception_C rv') \<noteq> NONE"
+      with Inl have
+        rv': "error_C (HEAP_DATA_exception_C.exception_C rv') \<noteq> NONE"
         unfolding R_HEAP_DATA_rel_def ERROR_rel_def by simp
       hence "?c rv' s'" by (simp add: NONE_def)
-      from Inl and rv' have "corres ?r \<top> (\<lambda>s'. ?r' rv (rv', s')) (return rv) (?t rv')"
+      from Inl and rv' have
+        "corres ?r \<top> (\<lambda>s'. ?r' rv (rv', s')) (return rv) (?t rv')"
         by (simp add: R_HEAP_DATA_rel_def R_STORED_DATA_rel_def)
       thus ?thesis using `?c rv' s'` by auto
     next
       let ?error = "error_C (HEAP_DATA_exception_C.exception_C rv')"
-      let ?data = "tdHEAP_DATA_C.data_C (HEAP_DATA_exception_C.value_C rv')"
-      let ?dataSize = "tdHEAP_DATA_C.dataSize_C (HEAP_DATA_exception_C.value_C rv')"
+      let ?data =
+        "tdHEAP_DATA_C.data_C (HEAP_DATA_exception_C.value_C rv')"
+      let ?dataSize = "tdHEAP_DATA_C.dataSize_C
+                         (HEAP_DATA_exception_C.value_C rv')"
       case (Inr v)
       fix s'
       assume "?r' rv (rv', s')"
-      with Inr have rv'_e: "?error = NONE" unfolding R_HEAP_DATA_rel_def ERROR_rel_def by simp
+      with Inr have rv'_e: "?error = NONE"
+        unfolding R_HEAP_DATA_rel_def ERROR_rel_def by simp
       hence "\<not>?c rv' s'" by (simp add: NONE_def)
       from Inr and `?r' rv (rv', s')` have rv'_v:
-        "HEAP_DATA_rel (E_STORED_DATA_rel string_rel) v (HEAP_DATA_exception_C.value_C rv', s')"
+        "HEAP_DATA_rel (E_STORED_DATA_rel string_rel) v
+           (HEAP_DATA_exception_C.value_C rv', s')"
         unfolding R_HEAP_DATA_rel_def by simp
       hence unpack: "\<forall>r \<in> fst (unpack_TPM_STORED_DATA12' ?data ?dataSize s').
           STORED_DATA_rel string_rel v r"
         unfolding HEAP_DATA_rel_def E_STORED_DATA_rel_def by simp
-      let ?r'' = "\<lambda>rv rv'. case rv of Inl e \<Rightarrow> False | Inr v \<Rightarrow> STORED_DATA_rel string_rel v rv'"
+      let ?r'' =
+        "\<lambda>rv rv'. case rv of Inl e \<Rightarrow> False
+                           | Inr v \<Rightarrow> STORED_DATA_rel string_rel v rv'"
       let ?unpack = "unpack_TPM_STORED_DATA12' ?data ?dataSize"
       have "corres ?r \<top> (\<lambda>s'. ?r' (Inr v) (rv', s')) (return (Inr v)) (?f rv')"
       apply (rule corres_bind_return)
       proof (rule corres_split' [where r'="?r''" and Q="\<top>\<top>" and Q'="\<top>\<top>"])
-        have p: "\<forall>(s, s') \<in> SR. ?r' (Inr v) (rv', s') \<longrightarrow> (\<forall>(r', t') \<in> fst (?unpack s').
-              \<exists>(r, t) \<in> fst (return (Inr v) s). (t, t') \<in> SR \<and> ?r'' r (r', t'))"
+        have p: "\<forall>(s, s') \<in> SR. ?r' (Inr v) (rv', s')
+                 \<longrightarrow> (\<forall>(r', t') \<in> fst (?unpack s').
+             \<exists>(r, t) \<in> fst (return (Inr v) s). (t, t') \<in> SR \<and> ?r'' r (r', t'))"
           unfolding R_HEAP_DATA_rel_def STORED_DATA_rel_def return_def by simp
         with no_fail_unpack_TPM_STORED_DATA12'
-          show "corres ?r'' \<top> (\<lambda>s'. ?r' (Inr v) (rv', s')) (return (Inr v)) ?unpack"
+        show "corres ?r'' \<top> (\<lambda>s'. ?r' (Inr v) (rv', s'))
+                (return (Inr v)) ?unpack"
           by (fast intro!: corres_no_failI)
       next
         show "\<And>rv rv'. corres ?r \<top> (\<lambda>s'. ?r'' rv (rv', s') \<and> True) (return rv)
           (return (TPM_STORED_DATA12_exception_C (tdEXCEPTION_C NONE) rv'))"
-          by (case_tac rv, auto simp add: R_STORED_DATA_rel_def STORED_DATA_rel_def)
+          by (case_tac rv,
+              auto simp add: R_STORED_DATA_rel_def STORED_DATA_rel_def)
       next show "\<lbrace>\<top>\<rbrace> return (Inr v) \<lbrace>\<top>\<top>\<rbrace>" by (rule hoare_post_taut)
-      next show "\<lbrace>\<lambda>s'. ?r' (Inr v) (rv', s')\<rbrace> ?unpack \<lbrace>\<top>\<top>\<rbrace>" by (rule hoare_post_taut)
+      next show "\<lbrace>\<lambda>s'. ?r' (Inr v) (rv', s')\<rbrace> ?unpack \<lbrace>\<top>\<top>\<rbrace>"
+          by (rule hoare_post_taut)
       qed
       thus ?thesis using Inr and `\<not>?c rv' s'` by simp
     qed
